chore: PoC of flushability

DataflowRewriter/Rewrites/JoinRewriteCorrect.lean
@@ -1,7 +1,7 @@
 /-
-Copyright (c) 2024 VCA Lab, EPFL. All rights reserved.
+Copyright (c) 2024-2025 VCA Lab, EPFL. All rights reserved.
 Released under Apache 2.0 license as described in the file LICENSE.
-Authors: Yann Herklotz
+Authors: Yann Herklotz, Hamza Remmal
 -/
 
 import Lean
@@ -10,6 +10,7 @@ import Qq
 
 import DataflowRewriter.Simp
 import DataflowRewriter.Module
+import DataflowRewriter.FlushedModule
 import DataflowRewriter.ModuleReduction
 import DataflowRewriter.ExprLow
 import DataflowRewriter.Component
@@ -31,6 +32,9 @@ namespace DataflowRewriter.JoinRewrite
 open StringModule
 
 abbrev Ident := Nat
+
+abbrev ExtRule (S: Type _) := (Σ T: Type _, S → T → S → Prop)
+abbrev IntRule (S: Type _) := S → S → Prop
 
 -- abbrev S₁ := "S1"
 -- abbrev S₂ := "S2"
@@ -93,14 +97,6 @@ reduction_by
   dsimp [ ExprHigh.uncurry, ExprLow.build_module_expr, ExprLow.build_module_type, ExprLow.build_module, ExprLow.build_module', toString]
   simp only [find?_join1_data, find?_join2_data]
   dsimp
---   skip
-  -- dsimp -failIfUnchanged [drunfold_defs, toString, reduceAssocListfind?, reduceListPartition]
-  -- dsimp -failIfUnchanged [reduceExprHighLower, reduceExprHighLowerProdTR, reduceExprHighLowerConnTR]
-  -- dsimp [ ExprHigh.uncurry, ExprLow.build_module_expr, ExprLow.build_module_type, ExprLow.build_module, ExprLow.build_module', toString]
-  -- simp only [find?_pure_data2, find?_join2_data2, find?_join2_data, find?_join1_data, find?_join1_data2]
-  -- dsimp
-
-def cast_module_type {α} {f : α → Type _} {s s' : Σ T, f T} (heq : s = s') : f s.1 = f s'.1 := by simp_all
 
 variable (T₁ T₂ T₃) in
 def_module lhsModule : StringModule (lhsModuleType T₁ T₂ T₃) :=
@@ -137,11 +133,47 @@ theorem sigma_rw_simp {S T : Type _} {m m' : Σ (y : Type _), S → y → T → 
   m.snd x v y ↔ m'.snd x ((cast_first h).mp v) y := by
   constructor <;> (intros; subst h; assumption)
 
-inductive partially
+---------------------------------------------------------------------------------------------------
+---
+---------------------------------------------------------------------------------------------------
+
+inductive at_least_single_internal: lhsModuleType T₁ T₂ T₃ -> Prop where
+| mk: ∀ v q₁ q₂ q₃ q₄, at_least_single_internal ⟨⟨v :: q₃, q₄⟩, ⟨q₁, q₂⟩⟩
+
+---------------------------------------------------------------------------------------------------
+------------------------------------------- FLUSHABILITY ------------------------------------------
+---------------------------------------------------------------------------------------------------
 
 inductive partially_flushed: lhsModuleType T₁ T₂ T₃ -> Prop where
 | lhs: ∀ lower arb, partially_flushed ⟨lower, [], arb⟩
 | rhs: ∀ lower arb, partially_flushed ⟨lower, arb, []⟩
+
+theorem pf_is_partially_flushed:
+  ∀ s, pf (lhsModule T₁ T₂ T₃) s → partially_flushed s :=
+by
+  intro ⟨s1, s2, s3⟩ hr; dsimp [lhsModuleType, lhsModule] at *
+  specialize hr ?r (by simp; rfl)
+  cases s2 <;> cases s3 <;> try constructor
+  exfalso
+  apply hr ⟨⟨_, _⟩, ⟨_, _⟩⟩
+  dsimp
+  iterate 6 (apply Exists.intro _)
+  and_intros <;> rfl
+
+theorem partially_flushed_is_pf:
+  ∀ s, partially_flushed s → pf (lhsModule T₁ T₂ T₃) s :=
+by
+  intro s h
+  cases h
+  all_goals
+    unfold pf
+    intros rule hᵣ _ h
+    simp [lhsModule] at hᵣ <;> subst hᵣ
+    simp at h
+
+---------------------------------------------------------------------------------------------------
+----------- BASE RELATION BETWEEN (rhsModuleType T₁ T₂ T₃) and (lhsModuleType T₁ T₂ T₃) -----------
+---------------------------------------------------------------------------------------------------
 
 def ψ (rhs : rhsModuleType T₁ T₂ T₃) (lhs : lhsModuleType T₁ T₂ T₃) : Prop :=
   let ⟨⟨j2l, j2r⟩, ⟨j1l, j1r⟩⟩ := lhs
@@ -150,8 +182,709 @@ def ψ (rhs : rhsModuleType T₁ T₂ T₃) (lhs : lhsModuleType T₁ T₂ T₃)
   (j2l.map Prod.snd ++ j1r = p.map ((Prod.snd ∘ Prod.fst)) ++ j2r'.map Prod.fst ++ j1l') ∧
   (j2r = p.map Prod.snd ++ j2r'.map Prod.snd ++ j1r')
 
+theorem ψ_holds_over_internals_spec:
+  ∀ i s s', ψ i s → existSR (lhsModule T₁ T₂ T₃).internals s s' → ψ i s' :=
+by
+  intro ⟨⟨_, _⟩, ⟨⟨_, _⟩, _⟩⟩ s s' Hψ E
+  induction E
+  . assumption
+  . rename_i init mid _ rule Hrule c _ Himpl
+    apply Himpl; clear Himpl
+    unfold lhsModule at Hrule; simp at Hrule
+    subst_vars
+    obtain ⟨_, _, _, _, _, _, _, _⟩ := c
+    let ⟨⟨_, _⟩, ⟨_, _⟩⟩ := init
+    let ⟨⟨_, _⟩, ⟨_, _⟩⟩ := mid
+    rename_i a _ _ _ _ _ b; simp at a b
+    obtain ⟨ ⟨_, _⟩, ⟨_, _⟩⟩ := a
+    obtain ⟨ ⟨_, _⟩ , ⟨_, _⟩⟩ := b
+    unfold ψ at *; simp at *
+    subst_vars
+    obtain ⟨ _, ⟨_, _⟩ ⟩ := Hψ
+    simp; and_intros <;> assumption
 
--- TODO: Can I write differently the lambda that extract the element from p's queue
+theorem ψ_holds_over_internals_impl:
+  ∀ i i' s, ψ i s → existSR (rhsModule T₁ T₂ T₃).internals i i' → ψ i' s :=
+by
+  intro i i' ⟨⟨_, _⟩, ⟨_, _⟩⟩ Hψ E
+  induction E
+  . assumption
+  . rename_i init mid _ rule Hrule c _ Himpl
+    apply Himpl; clear Himpl
+    unfold rhsModule at Hrule; simp at Hrule
+    cases Hrule <;> subst_vars
+    . obtain ⟨_, _, _, _, _, _, _, ⟨⟨⟨_, _⟩, _⟩, _⟩, ⟨_, _⟩, _⟩ := c
+      let ⟨⟨_, _⟩, ⟨_, _⟩⟩ := init
+      let ⟨⟨_, _⟩, ⟨_, _⟩⟩ := mid
+      unfold ψ at *; simp at *
+      rename_i synth1 synth2;
+      obtain ⟨_, _⟩ := synth1
+      obtain ⟨_, _⟩ := synth2
+      obtain ⟨_, _, _⟩ := Hψ
+      and_intros <;> subst_vars <;> try simp
+      . assumption
+      . rename_i synth1 _ _ _ _ _ _
+        rw [<- synth1]; subst_vars
+        assumption
+      . assumption
+    . obtain ⟨_, _, _, _, _, _, _, _, ⟨⟨⟨_, _⟩, _⟩, ⟨⟨_, _⟩, _⟩⟩⟩ := c
+      let ⟨⟨_, _⟩, ⟨_, _⟩⟩ := init
+      let ⟨⟨_, _⟩, ⟨_, _⟩⟩ := mid
+      unfold ψ at *; simp at *
+      rename_i synth1 synth2;
+      obtain ⟨_, _⟩ := synth1
+      obtain ⟨_, _⟩ := synth2
+      obtain ⟨_, _, _⟩ := Hψ
+      and_intros <;> subst_vars <;> simp
+      . assumption
+      . assumption
+
+theorem ψ_holds_over_internals: ∀ i i' s s',
+  ψ i s → existSR (rhsModule T₁ T₂ T₃).internals i i' → existSR (lhsModule T₁ T₂ T₃).internals s s' → ψ i' s' :=
+by
+  intros i i' s s' _ _ _
+  have: ψ i s' := by
+    apply ψ_holds_over_internals_spec <;> assumption
+  apply ψ_holds_over_internals_impl <;> assumption
+
+-- TODO: Can I get rid of this very specific theorem?
+theorem f: ∀ ident,
+  ((rhsModule T₁ T₂ T₃).outputs.getIO ident).fst = ((lhsModule T₁ T₂ T₃).outputs.getIO ident).fst :=
+by
+  have: MatchInterface (rhsModule T₁ T₂ T₃) (lhsModule T₁ T₂ T₃) := by infer_instance
+  exact this.output_types
+
+-- TODO: Can I get rid of this very specific theorem?
+theorem f'₂: ∀ ident,
+  ((rhsModule T₁ T₂ T₃).inputs.getIO ident).fst = ((lhsModule T₁ T₂ T₃).inputs.getIO ident).fst :=
+by
+  have: MatchInterface (rhsModule T₁ T₂ T₃) (lhsModule T₁ T₂ T₃) := by infer_instance
+  exact this.input_types
+
+theorem inputs_preserves_ψ: ∀ ident i₁ i₂ v s₁ s₂,
+  ψ i₁ s₁
+  → ((rhsModule T₁ T₂ T₃).inputs.getIO ident).snd i₁ v i₂
+  → ((lhsModule T₁ T₂ T₃).inputs.getIO ident).snd s₁ ((f'₂ ident).mp v) s₂
+  → ψ i₂ s₂ :=
+by
+  intro ident ⟨⟨_, _⟩, ⟨_, _⟩, _⟩ ⟨⟨_, _⟩, ⟨_, _⟩, _⟩ v ⟨⟨_, _⟩, ⟨_, _⟩⟩ ⟨⟨_, _⟩, ⟨_, _⟩⟩  h₁ h₂ h₃
+  by_cases HContains: (rhsModule T₁ T₂ T₃).inputs.contains ident
+  . simp [rhsModule] at HContains
+    rcases HContains with h | h | h <;> subst h <;> simp only [eq_mp_eq_cast, cast_eq] at h₃
+    . --
+      unfold lhsModule at h₃
+      rw [PortMap.rw_rule_execution] at h₃
+      simp at h₃
+      obtain ⟨⟨_, _⟩, _, _⟩ := h₃
+      --
+      unfold rhsModule at h₂
+      rw [PortMap.rw_rule_execution] at h₂
+      simp at h₂
+      obtain ⟨⟨_, _⟩, ⟨_, _⟩, _⟩ := h₂
+      --
+      obtain ⟨_, _, _⟩ := h₁
+      --
+      subst_vars
+      --
+      dsimp [ψ]
+      and_intros
+      . rw [<- List.append_assoc, <- List.append_assoc]
+        congr
+      . assumption
+      . rfl
+    . --
+      unfold lhsModule at h₃
+      rw [PortMap.rw_rule_execution] at h₃
+      simp at h₃
+      obtain ⟨⟨_, _⟩, _, _⟩ := h₃
+      --
+      --
+      unfold rhsModule at h₂
+      rw [PortMap.rw_rule_execution] at h₂
+      simp at h₂
+      obtain ⟨⟨⟨_, _⟩, _⟩, ⟨_, _⟩, _⟩ := h₂
+      --
+      obtain ⟨_, _, _⟩ := h₁
+      subst_vars
+      dsimp [ψ]
+      and_intros
+      . assumption
+      . rw [<- List.append_assoc, <- List.append_assoc]
+        congr
+      . rfl
+    . --
+      unfold lhsModule at h₃
+      rw [PortMap.rw_rule_execution] at h₃
+      simp at h₃
+      obtain ⟨⟨_, _⟩, _, _⟩ := h₃
+      --
+      --
+      unfold rhsModule at h₂
+      rw [PortMap.rw_rule_execution] at h₂
+      simp at h₂
+      obtain ⟨⟨⟨_, _⟩, _⟩, ⟨_, _⟩, _⟩ := h₂
+      --
+      obtain ⟨_, _, _⟩ := h₁
+      --
+      subst_vars
+      --
+      dsimp [ψ]
+      and_intros
+      . assumption
+      . assumption
+      . simp
+  . exfalso; exact (PortMap.getIO_not_contained_false h₂ HContains)
+
+theorem outputs_preserves_ψ: ∀ ident i₁ i₂ v s₁ s₂,
+  ψ i₁ s₁
+  → ((rhsModule T₁ T₂ T₃).outputs.getIO ident).snd i₁ v i₂
+  → ((lhsModule T₁ T₂ T₃).outputs.getIO ident).snd s₁ ((f ident).mp v) s₂
+  → ψ i₂ s₂ :=
+by
+  intro ident ⟨⟨_, _⟩, ⟨_, _⟩, _⟩ ⟨⟨_, _⟩, ⟨_, _⟩, _⟩ v ⟨⟨_, _⟩, ⟨_, _⟩⟩ ⟨⟨_, _⟩, ⟨_, _⟩⟩ h₁ h₂ h₃
+  by_cases HContains: ((rhsModule T₁ T₂ T₃).outputs.contains ident)
+  . simp [rhsModule] at HContains; subst HContains
+    unfold rhsModule at h₂
+    rw [PortMap.rw_rule_execution] at h₂; simp at h₂
+    simp at *
+    repeat
+      cases ‹_ ∧ _›
+    simp at *
+    cases ‹_ ∧ _›
+    subst_vars
+
+    dsimp [ψ]
+    and_intros
+    . simp at *; assumption
+    . simp at *; assumption
+    . simp at *; assumption
+  . exfalso; exact (PortMap.getIO_not_contained_false h₃ HContains)
+
+theorem f₆: ∀ ident i₁ i₂ v s₁,
+  ψ i₁ s₁
+  → pf ((lhsModule T₁ T₂ T₃)) s₁
+  → ((rhsModule T₁ T₂ T₃).outputs.getIO ident).snd i₁ v i₂
+  → at_least_single_internal s₁ :=
+by
+  intro ident ⟨⟨_, _⟩, ⟨_, _⟩, _⟩ ⟨⟨_, _⟩, ⟨_, _⟩, _⟩ v ⟨⟨_, _⟩, ⟨_, _⟩⟩ h₁ h₂ h₃
+  by_cases HContains: (rhsModule T₁ T₂ T₃).outputs.contains ident
+  .
+    simp [rhsModule] at HContains <;> subst HContains
+    --
+    unfold rhsModule at h₃
+    rw [PortMap.rw_rule_execution] at h₃
+    simp at h₃
+    obtain ⟨⟨_, _, _⟩, _, _⟩ := h₃
+    obtain ⟨_, _, _⟩ := h₁
+    subst_vars
+    --
+    apply pf_is_partially_flushed at h₂
+    cases h₂
+    . rename_i h₁ h₂
+      simp at h₁ h₂
+
+      sorry -- TODO: Reasoning about the length again?
+    . rename_i h₁ h₂
+      simp at h₁ h₂
+      sorry -- TODO: Reasoning about the length again?
+  . exfalso; exact (PortMap.getIO_not_contained_false h₃ HContains)
+
+-- move to have a reasoning about atleast one in internal
+-- we case only on once over queues that are in the top queue
+theorem f₅: ∀ ident i₁ i₂ v s₁,
+  ψ i₁ s₁
+  → at_least_single_internal s₁
+  → ((rhsModule T₁ T₂ T₃).outputs.getIO ident).snd i₁ v i₂
+  → ∃ s₂, ((lhsModule T₁ T₂ T₃).outputs.getIO ident).snd s₁ ((f ident).mp v) s₂ :=
+by
+  intro ident ⟨⟨_, _⟩, ⟨_, _⟩, _⟩ ⟨⟨_, _⟩, ⟨_, _⟩, _⟩ v s₁ h₁ h₂ h₃
+  by_cases HContains: (rhsModule T₁ T₂ T₃).outputs.contains ident
+  . simp [rhsModule] at HContains <;> subst HContains
+    simp only [eq_mp_eq_cast, cast_eq] -- remove the cast
+    --
+    unfold rhsModule at h₃
+    rw [PortMap.rw_rule_execution] at h₃
+    simp at h₃
+    obtain ⟨⟨_, _, _⟩, _, _⟩ := h₃
+    subst_vars
+    --
+    cases h₂
+    obtain ⟨_, _, _⟩ := h₁
+    apply Exists.intro ⟨⟨_, _⟩, ⟨_, _⟩⟩
+    unfold lhsModule
+    rw [PortMap.rw_rule_execution]
+    simp
+    and_intros
+    . rw [List.map_cons, List.map_cons] at *
+      simp at *
+      iterate 2
+        cases ‹_ ∧ _›
+      apply Prod.ext <;> assumption
+    . rfl
+    . rw [List.map_cons] at *; assumption
+    . rfl
+    . rfl
+  . exfalso; exact (PortMap.getIO_not_contained_false h₃ HContains)
+
+---------------------------------------------------------------------------------------------------
+-----------------
+---------------------------------------------------------------------------------------------------
+
+theorem lhs_can_always_flush:
+  ∀ s, ∃ s', existSR (lhsModule T₁ T₂ T₃).internals s s' ∧ partially_flushed s' :=
+by
+  intro ⟨⟨l1, l2⟩, ⟨l3, l4⟩⟩
+  induction l3 generalizing l1 l2 l4 with
+  | nil =>
+    apply Exists.intro
+    and_intros
+    . apply existSR_reflexive
+    . constructor
+  | cons x xs ih =>
+    cases l4
+    . apply Exists.intro
+      and_intros
+      . apply existSR_reflexive
+      . constructor
+    . rename_i head tail
+      specialize ih (l1 ++ [(x, head)]) l2 tail
+      obtain ⟨ ⟨⟨_, _⟩, ⟨_, _⟩⟩, _, _⟩ := ih
+      apply Exists.intro ⟨ ⟨ _, _ ⟩, _, _ ⟩
+      and_intros
+      . apply existSR.step _ ⟨ ⟨ _, _ ⟩, _, _ ⟩ _
+        . unfold lhsModule; simp; rfl
+        . repeat apply Exists.intro
+          and_intros <;> rfl
+        . assumption
+      . assumption
+
+theorem lhs_can_always_input:
+  ∀ ident s₁ v,
+  (lhsModule T₁ T₂ T₃).inputs.contains ident
+  → ∃ s₂, ((lhsModule T₁ T₂ T₃).inputs.getIO ident).snd s₁ v s₂ :=
+by
+  intro ident ⟨⟨q₁, q₂⟩, ⟨q₃, q₄⟩⟩ v h
+  simp [lhsModule] at h
+  rcases h with h | h | h <;> subst h
+  . have: ((lhsModule T₁ T₂ T₃).inputs.getIO { inst := InstIdent.top, name := "i_2" }).fst = T₃ := by
+      simp [lhsModule, PortMap.getIO]
+    use ⟨⟨q₁, q₂ ++ [(this.mp v)]⟩, ⟨q₃, q₄⟩⟩
+    dsimp [lhsModule]
+    rw [PortMap.rw_rule_execution]
+    simp
+  . have: ((lhsModule T₁ T₂ T₃).inputs.getIO { inst := InstIdent.top, name := "i_0" }).fst = T₁ := by
+      simp [lhsModule, PortMap.getIO]
+    use ⟨⟨q₁, q₂⟩, ⟨q₃ ++ [(this.mp v)], q₄⟩⟩
+    dsimp [lhsModule]
+    rw [PortMap.rw_rule_execution]
+    simp
+  . have: ((lhsModule T₁ T₂ T₃).inputs.getIO { inst := InstIdent.top, name := "i_1" }).fst = T₂ := by
+      simp [lhsModule, PortMap.getIO]
+    use ⟨⟨q₁, q₂⟩, ⟨q₃, q₄ ++ [(this.mp v)]⟩⟩
+    dsimp [lhsModule]
+    rw [PortMap.rw_rule_execution]
+    simp
+
+theorem flhs_can_always_input:
+  ∀ ident s₁ v,
+  (lhsModule T₁ T₂ T₃).inputs.contains ident
+  → ∃ s₂, ((flushed (lhsModule T₁ T₂ T₃)).inputs.getIO ident).snd s₁ v s₂ :=
+by
+  intro ident s₁ v _
+  have: ∃ s₂, ((lhsModule T₁ T₂ T₃).inputs.getIO ident).snd s₁ ((flushed_preserves_input_over_getIO (lhsModule T₁ T₂ T₃) ident).mp v) s₂ := by
+    apply lhs_can_always_input <;> assumption
+  obtain ⟨s₃, h⟩ := this
+  have: ∃ s', existSR (lhsModule T₁ T₂ T₃).internals s₃ s' ∧ partially_flushed s' := by
+    apply lhs_can_always_flush
+  have ⟨s₄, _, _⟩ := this
+  use s₄
+  have: (flushed (lhsModule T₁ T₂ T₃)).inputs.getIO ident = rflushed (lhsModule T₁ T₂ T₃) ((lhsModule T₁ T₂ T₃).inputs.getIO ident) := by
+    apply flushed_inputs_are_rflushed
+    apply PortMap.rule_contains at h
+    assumption
+  rw [sigma_rw this]
+  dsimp [rflushed]
+  use s₃
+  and_intros
+  . assumption
+  . assumption
+  . apply partially_flushed_is_pf <;> assumption
+
+---------------------------------------------------------------------------------------------------
+----------
+---------------------------------------------------------------------------------------------------
+
+theorem lengthify {T₁: Type _} (a b: List T₁): a = b → a.length = b.length := by
+  intro heq; rw [heq]
+
+theorem takify {T₁: Type _} (l: ℕ) (l₁ l₂: List T₁): l₁ = l₂ -> List.take l l₁ = List.take l l₂ := by
+  intro heq; rw [heq]
+
+theorem dropify {T₁: Type _} (l: ℕ) (l₁ l₂: List T₁): l₁ = l₂ -> List.drop l l₁ = List.drop l l₂ := by
+  intro heq; rw [heq]
+
+theorem product_is_list_zip {T₁ T₂: Type _} (x: List (T₁ × T₂)):
+  x = List.zip (List.map Prod.fst x) (List.map Prod.snd x) :=
+by
+  induction x with
+  | nil => simp
+  | cons head tail ih =>
+    simp only [List.map_cons, List.zip_cons_cons, <- ih]
+
+theorem append_iff {α} {a b c d : List α}:
+  a.length = c.length → (a ++ b = c ++ d ↔ a = c ∧ b = d) :=
+by
+  intro lengths
+  constructor
+  . intro h
+    and_intros
+    . replace h := congrArg (List.take a.length) h
+      rw [List.take_left, lengths, List.take_left] at h
+      assumption
+    . apply dropify a.length at h
+      rw [List.drop_left, lengths, List.drop_left] at h
+      assumption
+  . intro ⟨_, _⟩; subst_vars; rfl
+
+theorem bla {α : Type _} {a c : α} (b : List α) :
+  a ∈ b → c ∈ b → b.length = 1 → a = c :=
+by
+  intro ha hc hl
+  cases b with
+  | nil => exfalso; rw [List.length_nil] at hl; contradiction
+  | cons x xs => cases xs with
+    | nil =>
+      simp at *; subst_vars; rfl
+    | cons x' xs' =>
+      repeat rw [List.length_cons] at hl
+      rw [Nat.add_eq_right] at hl
+      rw [Nat.add_eq_zero] at hl
+      cases ‹ _ ∧ _ ›
+      contradiction
+
+---------------------------------------------------------------------------------------------------
+--------------------------------------- LHS SPECIFIC LEMMAS ---------------------------------------
+---------------------------------------------------------------------------------------------------
+
+theorem input_rules_deterministic: ∀ ident s₁ v s₂ s₃,
+  ((lhsModule T₁ T₂ T₃).inputs.getIO ident).snd s₁ v s₂
+  → ((lhsModule T₁ T₂ T₃).inputs.getIO ident).snd s₁ v s₃
+  → s₂ = s₃ :=
+by
+  intro ident ⟨⟨_ , _⟩, ⟨_ , _⟩⟩ _ ⟨⟨_ , _⟩, ⟨_ , _⟩⟩ ⟨⟨_ , _⟩, ⟨_ , _⟩⟩ h₁ h₂
+  by_cases HContains: ((lhsModule T₁ T₂ T₃).inputs.contains ident)
+  . simp [lhsModule] at HContains
+    rcases HContains with h | h | h <;> subst h
+    all_goals
+      dsimp [lhsModule] at h₁ h₂
+      rw [PortMap.rw_rule_execution] at h₁ h₂
+      dsimp at h₁ h₂
+      repeat
+        cases ‹_ ∧ _›
+        try simp at *
+        try subst_vars
+      rfl
+  . exfalso; exact (PortMap.getIO_not_contained_false (by assumption) HContains)
+
+theorem internal_rules_deterministic:
+  ∀ rule ∈ (lhsModule T₁ T₂ T₃).internals, ∀ s₁ s₂ s₃, rule s₁ s₂ → rule s₁ s₃ → s₂ = s₃ :=
+by
+  intro _ _ ⟨⟨_ , _⟩, ⟨_ , _⟩⟩ ⟨⟨_ , _⟩, ⟨_ , _⟩⟩ ⟨⟨_ , _⟩, ⟨_ , _⟩⟩ h₁ h₂
+  simp [lhsModule] at *
+  subst_vars
+  dsimp at h₁ h₂
+  obtain ⟨_, _, _, _, _, _, _⟩ := h₁
+  obtain ⟨_, _, _, _, _, _, _⟩ := h₂
+  repeat
+    cases ‹_ ∧ _›
+    try simp at *
+    try subst_vars
+  rfl
+
+theorem output_rules_deterministic: ∀ ident s₁ v s₂ s₃,
+  ((lhsModule T₁ T₂ T₃).outputs.getIO ident).snd s₁ v s₂
+  → ((lhsModule T₁ T₂ T₃).outputs.getIO ident).snd s₁ v s₃
+  → s₂ = s₃ :=
+by
+  intro ident ⟨⟨_ , _⟩, ⟨_ , _⟩⟩ _ ⟨⟨_ , _⟩, ⟨_ , _⟩⟩ ⟨⟨_ , _⟩, ⟨_ , _⟩⟩ h₁ h₂
+  by_cases HContains: ((lhsModule T₁ T₂ T₃).outputs.contains ident)
+  . simp [lhsModule] at HContains; subst HContains
+    dsimp [lhsModule] at h₁ h₂
+    rw [PortMap.rw_rule_execution] at h₁ h₂
+    dsimp at h₁ h₂
+    repeat
+      cases ‹_ ∧ _›
+      try simp at *
+      try subst_vars
+    rfl
+  . exfalso; exact (PortMap.getIO_not_contained_false (by assumption) HContains)
+
+theorem hamza₂: ∀ rule ∈ (lhsModule T₁ T₂ T₃).internals, ∀ ident s₁ v s₂ s₃,
+  ((lhsModule T₁ T₂ T₃).inputs.getIO ident).snd s₁ v s₂
+  → ∃ s₄, ((lhsModule T₁ T₂ T₃).inputs.getIO ident).snd s₃ v s₄ :=
+by
+  intro rule _ ident _ _ _ ⟨⟨_ , _⟩, ⟨_ , _⟩⟩ _
+  by_cases HContains: ((lhsModule T₁ T₂ T₃).inputs.contains ident)
+  . -- TODO: Extract it as it's own theorem
+    simp [lhsModule] at HContains
+    rcases HContains with h | h | h <;> subst h
+    all_goals
+      apply Exists.intro ⟨⟨_ , _⟩, ⟨_ , _⟩⟩
+      dsimp [lhsModule]
+      rw [PortMap.rw_rule_execution]
+      simp <;> and_intros <;> rfl
+  . exfalso; exact (PortMap.getIO_not_contained_false (by assumption) HContains)
+
+theorem hamza: ∀ ident s₁ v s₂ s₃,
+  existSR (lhsModule T₁ T₂ T₃).internals s₁ s₃
+  → ((lhsModule T₁ T₂ T₃).inputs.getIO ident).snd s₁ v s₂
+  → ∃ s₄, ((lhsModule T₁ T₂ T₃).inputs.getIO ident).snd s₃ v s₄ :=
+by
+  intros ident s₁ v s₂ s₃ h _
+  induction h generalizing s₂ with
+  | done => use s₂
+  | step init mid final rule _ _ _ ih =>
+    have: (∃ s₄, ((lhsModule T₁ T₂ T₃).inputs.getIO ident).snd mid v s₄) := by
+      apply hamza₂ <;> assumption
+    obtain ⟨s, h⟩ := this
+    specialize ih s
+    apply ih
+    assumption
+
+theorem b': ∀ rule ∈ (lhsModule T₁ T₂ T₃).internals, ∀ ident s₁ v s₂ s₃,
+  ((lhsModule T₁ T₂ T₃).outputs.getIO ident).snd s₁ v s₂
+  → rule s₁ s₃
+  → ∃ s₄, ((lhsModule T₁ T₂ T₃).outputs.getIO ident).snd s₃ v s₄ :=
+by
+  intro rule hᵣ ident ⟨⟨_ , _⟩, ⟨_ , _⟩⟩ v ⟨⟨_ , _⟩, ⟨_ , _⟩⟩ ⟨⟨_ , _⟩, ⟨_ , _⟩⟩ h₁ h₂
+  by_cases HContains: ((lhsModule T₁ T₂ T₃).outputs.contains ident)
+  . simp [lhsModule] at HContains
+    simp [lhsModule] at hᵣ
+    unfold lhsModule at h₁
+    rw [PortMap.rw_rule_execution] at h₁
+    subst_vars
+    dsimp at *
+    obtain ⟨_, _, _, _, _, _, ⟨⟨_ , _⟩ , _⟩, ⟨_ , _⟩, _⟩ := h₂
+    simp at *; subst_vars
+    repeat cases ‹_ ∧ _›
+    subst_vars; simp
+    -- extract this as it's own lemma
+    apply Exists.intro ⟨⟨_ , _⟩, ⟨_ , _⟩⟩
+    dsimp [lhsModule]
+    rw [PortMap.rw_rule_execution]
+    dsimp <;> and_intros <;> rfl
+  . exfalso; exact (PortMap.getIO_not_contained_false h₁ HContains)
+
+theorem b'': ∀ ident s₁ v s₂ s₃,
+  existSR (lhsModule T₁ T₂ T₃).internals s₁ s₃
+  → ((lhsModule T₁ T₂ T₃).outputs.getIO ident).snd s₁ v s₂
+  → ∃ s₄, ((lhsModule T₁ T₂ T₃).outputs.getIO ident).snd s₃ v s₄ :=
+by
+  intros ident s₁ v s₂ s₃ h _
+  induction h generalizing s₂ with
+  | done => use s₂
+  | step init mid final rule _ _ _ ih =>
+    have: (∃ s₄, ((lhsModule T₁ T₂ T₃).outputs.getIO ident).snd mid v s₄) := by
+      apply b' <;> assumption
+    obtain ⟨s, h⟩ := this
+    specialize ih s
+    apply ih
+    assumption
+
+theorem b'₄: ∀ rule ∈ (lhsModule T₁ T₂ T₃).internals, ∀ ident s₁ v s₂ s₃ s₄,
+  ((lhsModule T₁ T₂ T₃).outputs.getIO ident).snd s₁ v s₂
+  → rule s₁ s₃
+  → rule s₂ s₄
+  → ((lhsModule T₁ T₂ T₃).outputs.getIO ident).snd s₃ v s₄ :=
+by
+  intro rule h₁ ident ⟨⟨_ , _⟩, ⟨_ , _⟩⟩ _ ⟨⟨_ , _⟩, ⟨_ , _⟩⟩ ⟨⟨_ , _⟩, ⟨_ , _⟩⟩ ⟨⟨_ , _⟩, ⟨_ , _⟩⟩ h₂ h₃ h₄
+  by_cases HContains: ((lhsModule T₁ T₂ T₃).outputs.contains ident)
+  . -- process and unfold the fact that use the internal rule
+    simp [lhsModule] at h₁; subst h₁; dsimp at h₃ h₄
+    -- process the fact we use the output rule
+    simp [lhsModule] at HContains; subst HContains
+    dsimp [lhsModule] at h₂
+    rw [PortMap.rw_rule_execution] at h₂
+    dsimp at h₂
+    dsimp [lhsModule]
+    rw [PortMap.rw_rule_execution]
+    dsimp
+    obtain ⟨_, _, _, _, _, _, _⟩ := h₃
+    obtain ⟨_, _, _, _, _, _, _⟩ := h₄
+    repeat
+      cases ‹_ ∧ _›
+      try simp at *
+      try subst_vars
+    and_intros <;> rfl
+  . exfalso; exact (PortMap.getIO_not_contained_false (by assumption) HContains)
+
+theorem b'₃: ∀ rule ∈ (lhsModule T₁ T₂ T₃).internals, ∀ ident s₁ v s₂ s₃,
+  ((lhsModule T₁ T₂ T₃).outputs.getIO ident).snd s₁ v s₂
+  → rule s₁ s₃
+  → ∃ s₄, rule s₂ s₄ :=
+by
+  intro rule h₁ ident ⟨⟨_ , _⟩, ⟨_ , _⟩⟩ _ ⟨⟨_ , _⟩, ⟨_ , _⟩⟩ ⟨⟨_ , _⟩, ⟨_ , _⟩⟩ h₃ h₂
+  by_cases HContains: ((lhsModule T₁ T₂ T₃).outputs.contains ident)
+  . simp [lhsModule] at HContains; subst HContains
+    unfold lhsModule at h₃
+    rw [PortMap.rw_rule_execution] at h₃
+    dsimp at h₃
+    simp [lhsModule] at h₁; subst h₁
+    obtain ⟨_, _, _, _, _, _, ⟨⟨_ , _⟩ , _⟩, ⟨_ , _⟩, _⟩ := h₂
+    simp at *; subst_vars
+    repeat cases ‹ _ ∧ _ ›
+    subst_vars; simp
+    apply Exists.intro ⟨⟨_ , _⟩, ⟨_ , _⟩⟩; and_intros <;> rfl
+  . exfalso; exact (PortMap.getIO_not_contained_false (by assumption) HContains)
+
+theorem b₃: ∀ ident s₁ v s₂ s₃ s₄,
+  existSR (lhsModule T₁ T₂ T₃).internals s₁ s₃
+  → ((lhsModule T₁ T₂ T₃).outputs.getIO ident).snd s₁ v s₂
+  → ((lhsModule T₁ T₂ T₃).outputs.getIO ident).snd s₃ v s₄
+  → existSR (lhsModule T₁ T₂ T₃).internals s₂ s₄:=
+by
+  intros ident s₁ v s₂ s₃ s₄ h _ _
+  induction h generalizing s₂ with
+  | done =>
+    have: s₂ = s₄ := by
+      apply output_rules_deterministic <;> assumption
+    subst this
+    apply existSR_reflexive
+  | step init mid _ rule _ _ _ ih =>
+    have: (∃ mid', rule s₂ mid' ∧ existSR (lhsModule T₁ T₂ T₃).internals mid' s₄) := by
+      have: (∃ m, rule s₂ m) := by
+        apply b'₃ <;> assumption
+      obtain ⟨m, _⟩ := this
+      use m
+      and_intros
+      . assumption
+      . apply ih
+        . apply b'₄ _ _ _ init _ s₂ <;> assumption
+        . assumption
+    obtain ⟨mid', _, _⟩ := this
+    apply existSR_transitive _ _ mid'
+    . apply existSR_single_step <;> and_intros <;> assumption
+    . assumption
+
+theorem b'₅: ∀ rule ∈ (lhsModule T₁ T₂ T₃).internals, ∀ ident s₁ v s₂ s₃ s₄,
+  ((lhsModule T₁ T₂ T₃).inputs.getIO ident).snd s₁ v s₂
+  → ((lhsModule T₁ T₂ T₃).inputs.getIO ident).snd s₃ v s₄
+  → rule s₁ s₃
+  → rule s₂ s₄ :=
+by
+  intro rule hᵣ ident ⟨⟨_ , _⟩, ⟨_ , _⟩⟩ _ ⟨⟨_ , _⟩, ⟨_ , _⟩⟩ ⟨⟨_ , _⟩, ⟨_ , _⟩⟩ ⟨⟨_ , _⟩, ⟨_ , _⟩⟩ hᵢ hᵢ' hᵣ'
+  by_cases HContains: ((lhsModule T₁ T₂ T₃).inputs.contains ident)
+  . -- extract the names of the ports
+    simp [lhsModule] at HContains
+    -- work on the internal rules
+    simp [lhsModule] at hᵣ <;> subst hᵣ
+    obtain ⟨_, _, _, _, _, _, ⟨⟨_ , _⟩ , _⟩, ⟨_ , _⟩, _⟩ := hᵣ'
+    simp at * <;> (repeat cases ‹_ ∧ _›) <;> subst_vars
+    -- work on each input rule
+    rcases HContains with h | h | h <;> subst h
+    all_goals
+      dsimp [lhsModule] at hᵢ hᵢ'
+      rw [PortMap.rw_rule_execution] at hᵢ hᵢ'
+      dsimp at hᵢ hᵢ'
+      obtain ⟨⟨_ , _⟩, _, _⟩ := hᵢ
+      obtain ⟨⟨_ , _⟩, _, _⟩ := hᵢ'
+      subst_vars
+      simp
+  . exfalso; exact (PortMap.getIO_not_contained_false (by assumption) HContains)
+
+---------------------------------------------------------------------------------------------------
+-----------
+---------------------------------------------------------------------------------------------------
+
+-- TODO: Was called bll₂
+theorem flushed_preserves_input_over_getIO' {Ident S: Type _} [DecidableEq Ident] (mod: Module Ident S):
+  ∀ ident, (mod.inputs.getIO ident).fst = ((flushed mod).inputs.getIO ident).fst :=
+by
+  intro; symm; apply flushed_preserves_input_over_getIO
+
+theorem bll'₂ {Ident S: Type _} [DecidableEq Ident] (mod: Module Ident S): ∀ ident s₁ v s₂ s₃,
+  (mod.inputs.getIO ident).snd s₁ v s₂
+  → existSR (mod.internals) s₂ s₃
+  → pf mod s₃
+  → ((flushed mod).inputs.getIO ident).snd s₁ ((flushed_preserves_input_over_getIO' mod ident).mp v) s₃ :=
+by
+  intro ident s₁ v s₂ s₃ h₁ h₂ h₃
+  by_cases HContains: mod.inputs.contains ident
+  . have: (flushed mod).inputs.getIO ident = rflushed mod (mod.inputs.getIO ident) := by
+      apply flushed_inputs_are_rflushed <;> assumption
+    rw [sigma_rw this]
+    dsimp [rflushed]
+    use s₂
+    and_intros <;> simpa
+  . exfalso; exact (PortMap.getIO_not_contained_false (by assumption) HContains)
+
+theorem abc: ∀ ident s₁ v s₂,
+  ((lhsModule T₁ T₂ T₃).inputs.getIO ident).snd s₁ v s₂
+  → ∃ s₃, ((flushed (lhsModule T₁ T₂ T₃)).inputs.getIO ident).snd s₁ ((flushed_preserves_input_over_getIO' (lhsModule T₁ T₂ T₃) ident).mp v) s₃ :=
+by
+  intros ident _ _ s₂ _
+  have: ∃ s₃, existSR (lhsModule T₁ T₂ T₃).internals s₂ s₃ ∧ partially_flushed s₃ := by
+      apply lhs_can_always_flush s₂
+  obtain ⟨s₃, _, h⟩ := this
+  apply partially_flushed_is_pf at h
+  use s₃
+  apply bll'₂ <;> assumption
+
+theorem abc₃: ∀ ident s₁ v s₂ s₃,
+  ((lhsModule T₁ T₂ T₃).inputs.getIO ident).snd s₁ v s₂
+  → ((flushed (lhsModule T₁ T₂ T₃)).inputs.getIO ident).snd s₁ ((flushed_preserves_input_over_getIO' (lhsModule T₁ T₂ T₃) ident).mp v) s₃
+  → existSR (lhsModule T₁ T₂ T₃).internals s₂ s₃ :=
+by
+  intros _ s₁ _ s₂ s₃ _ h
+  apply flushed_reachable_from_nonflushed
+  . simp at *
+    assumption
+  . simp at *
+    assumption
+
+theorem bll'₃: ∀ ident s v s',
+  ((lhsModule T₁ T₂ T₃).inputs.getIO ident).snd s v s'
+  -> ∃ s'', ((flushed (lhsModule T₁ T₂ T₃)).inputs.getIO ident).snd s ((flushed_preserves_input_over_getIO' (lhsModule T₁ T₂ T₃) ident).mp v) s'' ∧ existSR ((lhsModule T₁ T₂ T₃).internals) s' s'' ∧ pf (lhsModule T₁ T₂ T₃) s'' :=
+by
+  intros ident s v _ _
+  have: ∃ s'', ((flushed (lhsModule T₁ T₂ T₃)).inputs.getIO ident).snd s ((flushed_preserves_input_over_getIO' (lhsModule T₁ T₂ T₃) ident).mp v) s'' := by
+    apply abc <;> assumption
+  obtain ⟨s₁, h⟩ := this
+  use s₁
+  and_intros <;> try assumption
+  . apply flushed_reachable_from_nonflushed
+    all_goals
+      simp at * -- TODO: Can I get rid of this simp?
+      assumption
+  . apply flushed_modules_has_flushed_states <;> assumption
+
+---------------------------------------------------------------------------------------------------
+-----
+---------------------------------------------------------------------------------------------------
+
+-- "if we pop an output from a flushed state, the resulting state is also flushed"
+theorem b₂: ∀ ident s₁ v s₂,
+  pf (lhsModule T₁ T₂ T₃) s₁
+  → ((lhsModule T₁ T₂ T₃).outputs.getIO ident).snd s₁ v s₂
+  →  pf (lhsModule T₁ T₂ T₃) s₂ :=
+by
+  intro ident ⟨⟨_ , _⟩, ⟨_ , _⟩⟩ _ ⟨⟨_ , _⟩, ⟨_ , _⟩⟩ hpf h₁
+  apply pf_is_partially_flushed at hpf
+  apply partially_flushed_is_pf
+  by_cases HContains: ((lhsModule T₁ T₂ T₃).outputs.contains ident)
+  . simp [lhsModule] at HContains <;> subst HContains
+    dsimp [lhsModule] at h₁
+    rw [PortMap.rw_rule_execution] at h₁
+    repeat
+      cases ‹_ ∧ _›; simp at *
+    subst_vars
+    cases hpf <;> constructor
+  . exfalso; exact (PortMap.getIO_not_contained_false (by assumption) HContains)
+
+---------------------------------------------------------------------------------------------------
+-------------------------- NON-FLUSHED, NON-INDUCTIVE ψ PROOF (BASELINE) --------------------------
+---------------------------------------------------------------------------------------------------
+
 def φ (rhs : rhsModuleType T₁ T₂ T₃) (lhs : lhsModuleType T₁ T₂ T₃) : Prop :=
   (ψ rhs lhs) ∧ (partially_flushed lhs)
 
@@ -210,159 +943,10 @@ theorem φ_indistinguishable :
         and_intros <;> try rfl
     . exfalso; exact (PortMap.getIO_not_contained_false H HContains)
 
-theorem something':
-  ∀ s, ∃ s', existSR (lhsModule T₁ T₂ T₃).internals s s' ∧ partially_flushed s' := by
-  intro ⟨⟨l1, l2⟩, ⟨l3, l4⟩⟩
-  induction l3 generalizing l1 l2 l4 with
-  | nil =>
-    apply Exists.intro
-    and_intros
-    . apply existSR_reflexive
-    . constructor
-  | cons x xs ih =>
-    cases l4
-    . apply Exists.intro
-      and_intros
-      . apply existSR_reflexive
-      . constructor
-    . rename_i head tail
-      specialize ih (l1 ++ [(x, head)]) l2 tail
-      obtain ⟨ ⟨⟨_, _⟩, ⟨_, _⟩⟩, HExists, HPartiallyFlushed⟩ := ih
-      apply Exists.intro ⟨ ⟨ _, _ ⟩, _, _ ⟩
-      and_intros
-      . apply existSR.step _ ⟨ ⟨ _, _ ⟩, _, _ ⟩ _
-        . unfold lhsModule; simp
-          rfl
-        . repeat apply Exists.intro
-          and_intros <;> rfl
-        . apply HExists
-      . assumption
-
-theorem something:
-  ∀ i s s', ψ i s → existSR (lhsModule T₁ T₂ T₃).internals s s' → ψ i s' := by
-  intro ⟨⟨_, _⟩, ⟨⟨_, _⟩, _⟩⟩ s s' Hψ E
-  induction E
-  . assumption
-  . rename_i init mid _ rule Hrule c _ Himpl
-    apply Himpl; clear Himpl
-    unfold lhsModule at Hrule; simp at Hrule
-    subst_vars
-    obtain ⟨_, _, _, _, _, _, _, _⟩ := c
-    let ⟨⟨_, _⟩, ⟨_, _⟩⟩ := init
-    let ⟨⟨_, _⟩, ⟨_, _⟩⟩ := mid
-    rename_i a _ _ _ _ _ b; simp at a b
-    obtain ⟨ ⟨_, _⟩, ⟨_, _⟩⟩ := a
-    obtain ⟨ ⟨_, _⟩ , ⟨_, _⟩⟩ := b
-    unfold ψ at *; simp at *
-    subst_vars
-    obtain ⟨ _, ⟨_, _⟩ ⟩ := Hψ
-    simp; and_intros <;> assumption
-
-theorem something'':
-  ∀ i i' s, ψ i s → existSR (rhsModule T₁ T₂ T₃).internals i i' → ψ i' s := by
-  intro i i' ⟨⟨_, _⟩, ⟨_, _⟩⟩ Hψ E
-  induction E
-  . assumption
-  . rename_i init mid _ rule Hrule c _ Himpl
-    apply Himpl; clear Himpl
-    unfold rhsModule at Hrule; simp at Hrule
-    cases Hrule <;> subst_vars
-    . obtain ⟨_, _, _, _, _, _, _, ⟨⟨⟨_, _⟩, _⟩, _⟩, ⟨_, _⟩, _⟩ := c
-      let ⟨⟨_, _⟩, ⟨_, _⟩⟩ := init
-      let ⟨⟨_, _⟩, ⟨_, _⟩⟩ := mid
-      unfold ψ at *; simp at *
-      rename_i synth1 synth2;
-      obtain ⟨_, _⟩ := synth1
-      obtain ⟨_, _⟩ := synth2
-      obtain ⟨_, _, _⟩ := Hψ
-      and_intros <;> subst_vars <;> try simp
-      . assumption
-      . rename_i synth1 _ _ _ _ _ _
-        rw [<- synth1]; subst_vars
-        assumption
-      . assumption
-    . obtain ⟨_, _, _, _, _, _, _, _, ⟨⟨⟨_, _⟩, _⟩, ⟨⟨_, _⟩, _⟩⟩⟩ := c
-      let ⟨⟨_, _⟩, ⟨_, _⟩⟩ := init
-      let ⟨⟨_, _⟩, ⟨_, _⟩⟩ := mid
-      unfold ψ at *; simp at *
-      rename_i synth1 synth2;
-      obtain ⟨_, _⟩ := synth1
-      obtain ⟨_, _⟩ := synth2
-      obtain ⟨_, _, _⟩ := Hψ
-      and_intros <;> subst_vars <;> simp
-      . assumption
-      . assumption
-
-theorem s' {T₁ T₂ T₃: Type _} (i i': rhsModuleType T₁ T₂ T₃) :
-  ∀ rule, rule ∈ (rhsModule T₁ T₂ T₃).internals ∧ rule i i' → existSR (rhsModule T₁ T₂ T₃).internals i i' := by
-    intro rule ⟨_, _⟩
-    apply existSR.step i i' i' rule
-    . assumption
-    . assumption
-    . exact existSR_reflexive
-
-theorem lengthify {T₁: Type _} (a b: List T₁): a = b → a.length = b.length := by
-  intro heq; rw [heq]
-
-theorem takify {T₁: Type _} (l: ℕ) (l₁ l₂: List T₁): l₁ = l₂ -> List.take l l₁ = List.take l l₂ := by
-  intro heq; rw [heq]
-
-theorem dropify {T₁: Type _} (l: ℕ) (l₁ l₂: List T₁): l₁ = l₂ -> List.drop l l₁ = List.drop l l₂ := by
-  intro heq; rw [heq]
-
-theorem product_is_list_zip {T₁ T₂: Type _} (x: List (T₁ × T₂)): x = List.zip (List.map Prod.fst x) (List.map Prod.snd x) := by
-  induction x with
-  | nil => simp
-  | cons head tail ih =>
-    simp only [List.map_cons, List.zip_cons_cons, <- ih]
-
-theorem append_iff {α} {a b c d : List α} : a.length = c.length → (a ++ b = c ++ d ↔ a = c ∧ b = d) := by
-  intro lengths
-  constructor
-  . intro h
-    and_intros
-    . replace h := congrArg (List.take a.length) h
-      rw [List.take_left, lengths, List.take_left] at h
-      assumption
-    . apply dropify a.length at h
-      rw [List.drop_left, lengths, List.drop_left] at h
-      assumption
-  . intro ⟨_, _⟩; subst_vars; rfl
-
--- example {T1 T2 T3} : ∀ s : lhsModuleType T1 T2 T3, (∀ r s', r ∈ (lhsModule T1 T2 T3).internals → ¬ r s s') →
-example {T1 T2 T3} : ∀ s : lhsModuleType T1 T2 T3, (¬ ∃ s' r, r ∈ (lhsModule T1 T2 T3).internals ∧ r s s') → (∀ r ∈ (lhsModule T1 T2 T3).internals, ∀ s', ¬ r s s') := by
-  intro s H r hr s' hrss
-  apply H
-  exists s', r
-
-example {T1 T2 T3} : ∀ s : lhsModuleType T1 T2 T3, (∀ r ∈ (lhsModule T1 T2 T3).internals, ∀ s', ¬ r s s') → partially_flushed s := by
-  intro ⟨s1, s2, s3⟩ hr; dsimp [lhsModuleType, lhsModule] at *
-  specialize hr _ (by simp; rfl)
-  cases s2 <;> cases s3 <;> try constructor
-  exfalso
-  apply hr ⟨⟨_, _⟩, ⟨_, _⟩⟩
-  iterate 6 (apply Exists.intro _)
-  and_intros <;> dsimp
-
--- lhsModule is spec is trivial, because you just do the same steps as lhsModule'
--- lhsModule' being spec is not trivial
--- rhsModule' ⊑ lshModule' could be interesting, not sure if easier.
-def lhsModule' : StringModule (lhsModuleType T₁ T₂ T₃) :=
-  {
-    inputs := (lhsModule T₁ T₂ T₃).inputs.mapVal (λ k v =>
-        ⟨v.1, fun s ret s'' =>
-          ∃ (s' : lhsModuleType T₁ T₂ T₃), v.2 s ret s'
-            ∧ existSR (lhsModule T₁ T₂ T₃).internals s' s''                -- Allow rule executions
-            ∧ (∀ r ∈ (lhsModule T₁ T₂ T₃).internals, ∀ s_n, ¬ r s'' s_n)⟩  -- Ensure they are terminal
-      ),
-    outputs := (lhsModule T₁ T₂ T₃).outputs,
-    init_state := fun _ => True,
-  }
-
-theorem refines {T: Type _} [DecidableEq T]: rhsModule T₁ T₂ T₃ ⊑_{φ} lhsModule T₁ T₂ T₃ := by
-  unfold Module.refines_φ
+theorem refines₀: rhsModule T₁ T₂ T₃ p⊑_{φ} lhsModule T₁ T₂ T₃ := by
+  unfold Module.prefines_φ
   intro init_i init_s Hφ
-  apply Module.comp_refines.mk
+  apply Module.pcomp_refines.mk
   -- input rules
   . intro ident i s a
     by_cases HContains: ((rhsModule T₁ T₂ T₃).inputs.contains ident)
@@ -383,13 +967,13 @@ theorem refines {T: Type _} [DecidableEq T]: rhsModule T₁ T₂ T₃ ⊑_{φ} l
           rw [PortMap.rw_rule_execution (by dsimp [reducePortMapgetIO])]
           simp
         . -- verify that the invariant holds when we flush the system
-          obtain ⟨s', ⟨_, _⟩⟩ := something' ⟨⟨sj2l, sj2r⟩, sj1l ++ [heq.mp s], sj1r⟩ -- We flush the system to reach s'
+          obtain ⟨s', ⟨_, _⟩⟩ := lhs_can_always_flush ⟨⟨sj2l, sj2r⟩, sj1l ++ [heq.mp s], sj1r⟩ -- We flush the system to reach s'
           use s'
           apply And.intro
           . assumption
           . unfold φ at *
             apply And.intro
-            . apply something _ (⟨sj2l, sj2r⟩, sj1l ++ [heq.mp s], sj1r) s'
+            . apply ψ_holds_over_internals_spec _ (⟨sj2l, sj2r⟩, sj1l ++ [heq.mp s], sj1r) s'
               . obtain ⟨Hψ, _⟩ := Hφ
                 unfold ψ at *; simp at *
                 obtain ⟨_, _, _⟩ := Hψ
@@ -407,13 +991,13 @@ theorem refines {T: Type _} [DecidableEq T]: rhsModule T₁ T₂ T₃ ⊑_{φ} l
         use ⟨⟨sj2l, sj2r⟩, ⟨sj1l, sj1r ++ [s]⟩⟩
         apply And.intro
         . rw [PortMap.rw_rule_execution (by dsimp [reducePortMapgetIO])]; simp
-        . obtain ⟨s', ⟨_, _⟩⟩ := something' ⟨⟨sj2l, sj2r⟩, sj1l, sj1r ++ [s]⟩
+        . obtain ⟨s', ⟨_, _⟩⟩ := lhs_can_always_flush ⟨⟨sj2l, sj2r⟩, sj1l, sj1r ++ [s]⟩
           use s'
           apply And.intro
           . assumption
           . unfold φ at *
             apply And.intro
-            . apply something _ (⟨sj2l, sj2r⟩, sj1l, sj1r ++ [s]) s'
+            . apply ψ_holds_over_internals_spec _ (⟨sj2l, sj2r⟩, sj1l, sj1r ++ [s]) s'
               . obtain ⟨Hψ, _⟩ := Hφ
                 unfold ψ at *; simp at *
                 obtain ⟨_, _, _⟩ := Hψ
@@ -431,13 +1015,13 @@ theorem refines {T: Type _} [DecidableEq T]: rhsModule T₁ T₂ T₃ ⊑_{φ} l
         use ⟨⟨sj2l, sj2r ++ [s]⟩, ⟨sj1l, sj1r⟩⟩
         apply And.intro
         . rw [PortMap.rw_rule_execution (by dsimp [reducePortMapgetIO])]; simp
-        . obtain ⟨s', ⟨_, _⟩⟩ := something' ⟨⟨sj2l, sj2r ++ [s]⟩, sj1l, sj1r⟩
+        . obtain ⟨s', ⟨_, _⟩⟩ := lhs_can_always_flush ⟨⟨sj2l, sj2r ++ [s]⟩, sj1l, sj1r⟩
           use s'
           apply And.intro
           . assumption
           . unfold φ at *
             apply And.intro
-            . apply something _ (⟨sj2l, sj2r  ++ [s]⟩, sj1l, sj1r) s'
+            . apply ψ_holds_over_internals_spec _ (⟨sj2l, sj2r  ++ [s]⟩, sj1l, sj1r) s'
               . obtain ⟨Hψ, _⟩ := Hφ
                 unfold ψ at *; simp at *
                 obtain ⟨_, _, _⟩ := Hψ
@@ -538,12 +1122,436 @@ theorem refines {T: Type _} [DecidableEq T]: rhsModule T₁ T₂ T₃ ⊑_{φ} l
     . unfold φ at *
       obtain ⟨_, _⟩ := Hφ
       apply And.intro
-      . apply (something'' init_i)
+      . apply ψ_holds_over_internals_impl init_i
         . assumption
-        . apply s' init_i mid_i rule
-          and_intros <;> assumption
+        . apply existSR_single_step' <;> assumption
       . assumption
 
-#print axioms refines
+---------------------------------------------------------------------------------------------------
+--------------- FORANY MODULE, IT'S FLUSHED VERSION REFINES THE NON-FLUSHED VERSION ---------------
+---------------------------------------------------------------------------------------------------
+
+theorem refines₁ {Ident S: Type _} [DecidableEq Ident] (mod: Module Ident S): flushed mod p⊑_{Eq} mod := by
+  unfold Module.prefines_φ
+  intro init_i init_s Hφ
+  subst_vars
+  apply Module.pcomp_refines.mk
+  -- input rules
+  . intro _ mid_i v h
+    apply bll at h
+    obtain ⟨s', _, _⟩ := h
+    use s', mid_i
+  -- output rules
+  . intro _ mid_i _ _
+    use mid_i
+    and_intros
+    . simp only [flushed, eq_mp_eq_cast, cast_eq] at *
+      assumption
+    . rfl
+  -- internal rules
+  . intro _ mid_i _ _
+    use mid_i
+    and_intros
+    . apply existSR.step
+      . simp only [flushed, List.not_mem_nil] at *
+      . assumption
+      . apply existSR_reflexive
+    . rfl
+
+---------------------------------------------------------------------------------------------------
+------------------- FLUSHED, INDUCTIVE, OVER LHS PROOF THAT (LHS ⊑ FLUSHED LHS) -------------------
+---------------------------------------------------------------------------------------------------
+
+def φ₂ {Ident S: Type _} (mod: Module Ident S)(lhs : S) (rhs : S) : Prop :=
+  existSR mod.internals lhs rhs ∧ pf mod rhs
+
+theorem refines₂:
+  lhsModule T₁ T₂ T₃ p⊑_{φ₂ (lhsModule T₁ T₂ T₃)} flushed (lhsModule T₁ T₂ T₃) :=
+by
+  unfold Module.prefines_φ
+  intro init_i init_s ⟨Hφ, hpf⟩
+  apply Module.pcomp_refines.mk <;> unfold φ₂ at *
+  -- input rules
+  . intro ident mid_i v h
+    induction Hφ generalizing mid_i with
+    | done =>
+      apply bll'₃ at h
+      obtain ⟨s, _, _, _⟩ := h
+      use s, s
+      and_intros <;> try assumption
+      apply existSR_reflexive
+    | step init mid _ rule _ _ _ ih =>
+      specialize ih (by assumption)
+      have: ∃ s, ((lhsModule T₁ T₂ T₃).inputs.getIO ident).snd mid v s := by
+        apply hamza <;> try assumption
+        apply existSR_single_step <;> and_intros <;> assumption
+      obtain ⟨s, _⟩ := this
+      specialize ih s (by assumption)
+      obtain ⟨s₁, s₂, _, _, _, _⟩ := ih
+      use s₁, s₂
+      and_intros <;> try assumption
+      rename_i a _ _
+      dsimp [flushed] at a
+      apply existSR_norules at a; subst a
+      have: rule mid_i s := by apply b'₅ <;> assumption
+      apply (existSR_single_step' (lhsModule T₁ T₂ T₃).internals) at this <;> try assumption
+      apply existSR_transitive (lhsModule T₁ T₂ T₃).internals _ s <;> assumption
+  -- output rules
+  . intro _ mid_i _ h
+    dsimp [flushed] at *
+    apply b'' at Hφ
+    specialize Hφ h
+    obtain ⟨mid_s, _⟩ := Hφ
+    use mid_s
+    and_intros <;> try assumption
+    . apply b₃ <;> assumption
+    . apply b₂ <;> assumption
+  -- internal rules
+  . intros rule mid_i HRuleInInternal _
+    use init_s
+    and_intros
+    . apply existSR_reflexive
+    . cases Hφ with
+      | done =>
+        unfold pf at hpf
+        specialize hpf rule (by exact HRuleInInternal) mid_i
+        contradiction
+      | step _ mid _ rule' _ _ _ =>
+          have: rule = rule' := by
+            apply bla at HRuleInInternal
+            specialize HRuleInInternal (by assumption) (by dsimp[lhsModule])
+            assumption
+          subst this
+          have: mid_i = mid := by
+            apply internal_rules_deterministic <;> assumption
+          subst this <;> assumption
+    . assumption
+
+---------------------------------------------------------------------------------------------------
+---------
+---------------------------------------------------------------------------------------------------
+
+inductive empty_internal: lhsModuleType T₁ T₂ T₃ -> Prop where
+| mk: ∀ q₁ q₂ q₃, empty_internal ⟨⟨[], q₃⟩, ⟨q₁, q₂⟩⟩
+
+inductive single_internal: lhsModuleType T₁ T₂ T₃ -> Prop where
+| mk: ∀ v q₁ q₂ q₃, single_internal ⟨⟨[v], q₃⟩, ⟨q₁, q₂⟩⟩
+
+theorem f': ∀ s₁ s₂, ∀ rule ∈ (lhsModule T₁ T₂ T₃).internals,
+  empty_internal s₁
+  → rule s₁ s₂
+  → single_internal s₂ :=
+by
+  intro ⟨⟨_, _⟩,⟨_, _⟩⟩ ⟨⟨_, _⟩,⟨_, _⟩⟩ rule h₁ h₂ h₃
+  simp [lhsModule] at h₁
+  subst h₁
+
+  cases h₂
+  dsimp at h₃
+  simp at h₃
+  obtain ⟨_, _, _, _, _, _, _⟩ := h₃
+  repeat
+    cases ‹_ ∧ _›
+  subst_vars
+  rw [List.nil_append]
+  constructor
+
+theorem f₃: ∀ ident s₁ s₂ v,
+  single_internal s₁
+  → ((lhsModule T₁ T₂ T₃).outputs.getIO ident).snd s₁ v s₂
+  → empty_internal s₂ :=
+by
+  intro ident ⟨⟨_, _⟩,⟨_, _⟩⟩ ⟨⟨_, _⟩,⟨_, _⟩⟩ _ h₁ h₂
+  by_cases HContains: ((lhsModule T₁ T₂ T₃).outputs.contains ident)
+  . -- fetch the single output port ident
+    simp [lhsModule] at HContains; subst HContains
+    unfold lhsModule at h₂
+    rw [PortMap.rw_rule_execution] at h₂
+    dsimp at h₂
+    simp at h₂
+    repeat
+      cases ‹_ ∧ _›
+    subst_vars
+    cases h₁
+    constructor
+  . exfalso; exact (PortMap.getIO_not_contained_false (by assumption) HContains)
+
+---------------------------------------------------------------------------------------------------
+---------
+---------------------------------------------------------------------------------------------------
+
+def φ₃ (rhs : rhsModuleType T₁ T₂ T₃) (lhs : lhsModuleType T₁ T₂ T₃) :=
+  ψ rhs lhs ∧ empty_internal lhs
+
+theorem f₁: ∀ ident i₁ i₂ v s₁, ∀ rule ∈ (lhsModule T₁ T₂ T₃).internals,
+  φ₃ i₁ s₁
+  → ((rhsModule T₁ T₂ T₃).outputs.getIO ident).snd i₁ v i₂
+  → ∃ s₂, rule s₁ s₂ :=
+by
+  intro ident ⟨⟨_, _⟩,⟨_, _⟩⟩ ⟨⟨_, _⟩,⟨_, _⟩⟩ v ⟨⟨_, _⟩,⟨_, _⟩⟩ rule h₁ h₂ h₃
+  by_cases HContains: ((rhsModule T₁ T₂ T₃).outputs.contains ident)
+  . -- Fetch the output rule
+    simp [rhsModule] at HContains; subst HContains
+    obtain ⟨hψ, h₂⟩ := h₂
+    cases h₂
+    dsimp [ψ] at hψ
+    obtain ⟨_, _, _⟩ := hψ
+    subst_vars
+    -- work on h₃
+    unfold rhsModule at h₃
+    rw [PortMap.rw_rule_execution] at h₃
+    simp at h₃
+    repeat
+      cases ‹_ ∧ _›
+    subst_vars
+    -- work on h₁
+    simp [lhsModule] at h₁; subst h₁
+    dsimp
+    apply Exists.intro ⟨⟨_, _⟩,⟨_, _⟩⟩
+    repeat
+      apply Exists.intro
+    simp
+    and_intros <;> rfl
+  . exfalso; exact (PortMap.getIO_not_contained_false (by assumption) HContains)
+
+theorem f'': ∀ ident i₁ i₂ v s₁,
+  ψ i₁ s₁
+  → single_internal s₁
+  → ((rhsModule T₁ T₂ T₃).outputs.getIO ident).snd i₁ v i₂
+  → ∃ s₂, ((lhsModule T₁ T₂ T₃).outputs.getIO ident).snd s₁ ((f ident).mp v) s₂ :=
+by
+  intro ident ⟨⟨_, _⟩,⟨_, _⟩⟩ ⟨⟨_, _⟩,⟨_, _⟩⟩ _ ⟨⟨_, _⟩,⟨_, _⟩⟩ h₁ h₂ h₃
+  by_cases HContains: ((rhsModule T₁ T₂ T₃).outputs.contains ident)
+  . simp [rhsModule] at HContains; subst HContains
+    unfold rhsModule at h₃; rw [PortMap.rw_rule_execution] at h₃; simp at h₃
+    cases h₂
+    dsimp [ψ] at h₁
+    repeat
+      cases ‹_ ∧ _›
+    subst_vars
+    unfold lhsModule
+    apply Exists.intro ⟨⟨_, _⟩,⟨_, _⟩⟩
+    rw [PortMap.rw_rule_execution]; dsimp
+    and_intros
+    . simp at *
+      iterate 2 cases ‹_ ∧ _›
+      and_intros
+      . apply Prod.ext <;> assumption
+      . rfl
+    . rfl
+    . rfl
+  . exfalso; exact (PortMap.getIO_not_contained_false (by assumption) HContains)
+
+theorem refines₃: rhsModule T₁ T₂ T₃ ⊑_{φ₃} lhsModule T₁ T₂ T₃ := by
+  unfold Module.refines_φ
+  intro init_i init_s Hψ
+  apply Module.comp_refines.mk
+  -- input rules
+  . intro ident i s a
+    by_cases HContains: ((rhsModule T₁ T₂ T₃).inputs.contains ident)
+    . obtain ⟨⟨sj2l, sj2r⟩, ⟨sj1l, sj1r⟩⟩ := init_s
+      obtain ⟨⟨_, _⟩, ⟨_, _⟩, _⟩ := init_i
+      obtain ⟨⟨_, _⟩, ⟨_, _⟩, _⟩ := i
+
+      unfold rhsModule at HContains; simp at HContains
+      rcases HContains with h | h | h <;> subst_vars <;> simp
+      . unfold rhsModule at a
+        rw [PortMap.rw_rule_execution] at a
+        dsimp at a
+        obtain ⟨⟨_, _⟩, ⟨_, _⟩⟩ := a
+        subst_vars
+        have_hole heq : ((rhsModule T₁ T₂ T₃).inputs.getIO { inst := InstIdent.top, name := "i_0" }).fst = _ := by dsimp [reducePortMapgetIO]
+        -- We construct the almost_mid_s manually
+        use ⟨⟨sj2l, sj2r⟩, ⟨sj1l ++ [heq.mp s], sj1r⟩⟩
+        apply And.intro
+        . -- verify that the rule holds
+          rw [PortMap.rw_rule_execution (by dsimp [reducePortMapgetIO])]
+          simp -- TODO: Remove this simp here
+        . -- verify that the invariant holds when we flush the system
+          use ⟨⟨sj2l, sj2r⟩, sj1l ++ [heq.mp s], sj1r⟩
+          apply And.intro
+          . apply existSR_reflexive
+          . dsimp [φ₃, ψ] at Hψ
+            obtain ⟨⟨h, _, _⟩, hₑ⟩ := Hψ
+            dsimp [φ₃, ψ]
+            and_intros
+            . rw [<- List.append_assoc, <- List.append_assoc, h]
+            . assumption
+            . assumption
+            . cases hₑ; constructor
+      . unfold rhsModule at a
+        rw [PortMap.rw_rule_execution] at a
+        dsimp at a
+        obtain ⟨⟨⟨_, _⟩, _⟩, ⟨_, _⟩⟩ := a
+        subst_vars
+        have_hole heq : ((rhsModule T₁ T₂ T₃).inputs.getIO { inst := InstIdent.top, name := "i_1" }).fst = _ := by dsimp [reducePortMapgetIO]
+        use ⟨⟨sj2l, sj2r⟩, ⟨sj1l, sj1r ++ [heq.mp s]⟩⟩
+        apply And.intro
+        . rw [PortMap.rw_rule_execution (by dsimp [reducePortMapgetIO])]; simp
+        . use ⟨⟨sj2l, sj2r⟩, sj1l, sj1r ++ [heq.mp s]⟩
+          apply And.intro
+          . apply existSR_reflexive
+          . dsimp [φ₃, ψ] at Hψ
+            obtain ⟨⟨_, h, _⟩, hₑ⟩ := Hψ
+            subst_vars
+            dsimp [φ₃, ψ]
+            and_intros
+            . assumption
+            . rw [<- List.append_assoc, <- List.append_assoc, h]
+            . rfl
+            . cases hₑ; constructor
+      . unfold rhsModule at a
+        rw [PortMap.rw_rule_execution] at a
+        dsimp at a
+        obtain ⟨⟨⟨_, _⟩, _⟩, ⟨_, _⟩⟩ := a
+        subst_vars
+        have_hole heq : ((rhsModule T₁ T₂ T₃).inputs.getIO { inst := InstIdent.top, name := "i_2" }).fst = _ := by dsimp [reducePortMapgetIO]
+        use ⟨⟨sj2l, sj2r ++ [heq.mp s]⟩, ⟨sj1l, sj1r⟩⟩
+        apply And.intro
+        . rw [PortMap.rw_rule_execution (by dsimp [reducePortMapgetIO])]; simp
+        . use ⟨⟨sj2l, sj2r ++ [heq.mp s]⟩, sj1l, sj1r⟩
+          apply And.intro
+          . apply existSR_reflexive
+          . dsimp [φ₃, ψ] at Hψ
+            obtain ⟨⟨_, _, _⟩, hₑ⟩ := Hψ
+            subst_vars
+            dsimp [φ₃, ψ]
+            and_intros
+            . assumption
+            . assumption
+            . rw [<- List.append_assoc]
+            . cases hₑ; constructor
+    . exfalso; exact (PortMap.getIO_not_contained_false a HContains)
+  -- output rules
+  . intro ident i v hrule
+    by_cases HContains: ((rhsModule T₁ T₂ T₃).outputs.contains ident)
+    . have: ∃ rule, rule ∈ (lhsModule T₁ T₂ T₃).internals := by
+        simp [lhsModule]
+      obtain ⟨rule, h⟩ := this
+      have: ∃ almost_mid_s, rule init_s almost_mid_s := by
+        apply (f₁ _ init_i i) at Hψ
+        . specialize Hψ hrule
+          assumption
+        . assumption
+      obtain ⟨almost_mid_s, _⟩ := this
+      use almost_mid_s
+      rw [exists_and_left]
+      and_intros
+      . apply existSR_single_step' <;> assumption
+      . unfold φ₃ at Hψ
+        obtain ⟨_, _⟩ := Hψ
+        have hₛ: single_internal almost_mid_s := by
+          apply f' <;> assumption
+        have: existSR (lhsModule T₁ T₂ T₃).internals init_s almost_mid_s := by
+          apply existSR_single_step' <;> assumption
+        have hψ: ψ init_i almost_mid_s := by
+          apply ψ_holds_over_internals_spec <;> assumption
+        clear this
+        have: ∃ mid_s, ((lhsModule T₁ T₂ T₃).outputs.getIO ident).snd almost_mid_s ((f ident).mp v) mid_s := by
+          apply f'' <;> assumption
+        obtain ⟨mid_s, _⟩ := this
+        use mid_s
+        apply And.intro
+        . assumption
+        . unfold φ₃
+          apply And.intro
+          . apply outputs_preserves_ψ <;> assumption
+          . apply f₃ <;> assumption
+    . exfalso; exact (PortMap.getIO_not_contained_false hrule HContains)
+  -- internal rules
+  . intros
+    use init_s
+    apply And.intro
+    . exact existSR_reflexive
+    . dsimp [φ₃] at *
+      obtain ⟨_, _⟩ := Hψ
+      . apply And.intro
+        . apply ψ_holds_over_internals_impl init_i
+          . assumption
+          . apply existSR_single_step' <;> assumption
+        . assumption
+
+---------------------------------------------------------------------------------------------------
+
+def cast:
+  ∀ ident, ((flushed (rhsModule T₁ T₂ T₃)).inputs.getIO ident).fst = ((flushed (lhsModule T₁ T₂ T₃)).inputs.getIO ident).fst :=
+by
+  intro ident
+  have: MatchInterface (flushed (rhsModule T₁ T₂ T₃)) (rhsModule T₁ T₂ T₃) := by infer_instance
+  rw [this.input_types ident]
+  have: MatchInterface (flushed (lhsModule T₁ T₂ T₃)) (lhsModule T₁ T₂ T₃) := by infer_instance
+  rw [this.input_types ident]
+  have: MatchInterface (rhsModule T₁ T₂ T₃) (lhsModule T₁ T₂ T₃) := by infer_instance
+  exact this.input_types ident
+
+def cast':
+  ∀ ident, ((flushed (rhsModule T₁ T₂ T₃)).outputs.getIO ident).fst = ((flushed (lhsModule T₁ T₂ T₃)).outputs.getIO ident).fst :=
+by
+  dsimp [flushed]
+  have: MatchInterface (rhsModule T₁ T₂ T₃) (lhsModule T₁ T₂ T₃) := by infer_instance
+  exact this.output_types
+
+def φ₄ (rhs : rhsModuleType T₁ T₂ T₃) (lhs : lhsModuleType T₁ T₂ T₃) : Prop :=
+  ψ rhs lhs ∧ pf (lhsModule T₁ T₂ T₃) lhs
+
+-- TODO: Can I use only ψ?
+theorem refines₄:
+  flushed (rhsModule T₁ T₂ T₃) ⊑_{φ₄} flushed (lhsModule T₁ T₂ T₃) :=
+by
+  unfold Module.refines_φ
+  intro init_i init_s Hψ
+  apply Module.comp_refines.mk
+  . -- inputs rules
+    intro ident mid_i v h₁
+    have: ∃ s', ((flushed (lhsModule T₁ T₂ T₃)).inputs.getIO ident).snd init_s ((cast ident).mp v) s' := by
+      apply flhs_can_always_input
+      have: MatchInterface (rhsModule T₁ T₂ T₃) (lhsModule T₁ T₂ T₃) := by infer_instance
+      apply PortMap.rule_contains at h₁
+      rw [flushed_preserves_ports] at h₁
+      sorry -- trivial
+    obtain ⟨s', h₂⟩ := this
+    use s', s'
+    apply And.intro
+    . assumption
+    . apply And.intro
+      . apply existSR_reflexive
+      . unfold φ₄; apply And.intro
+        . apply bll at h₁
+          apply bll at h₂
+          obtain ⟨s₁, _, _⟩ := h₁
+          obtain ⟨s₂, _, _⟩ := h₂
+          simp at *
+          obtain ⟨_, _⟩ := Hψ
+          have: ψ s₁ s₂ := by
+            apply inputs_preserves_ψ <;> simpa
+          apply ψ_holds_over_internals <;> assumption
+        . apply flushed_modules_has_flushed_states <;> assumption
+  . -- outputs rules
+    intro ident mid_i v h₁
+    use init_s
+    rw [exists_and_left]
+    apply And.intro
+    . apply existSR_reflexive
+    . obtain ⟨_, _⟩ := Hψ
+      have: ∃ s', ((flushed (lhsModule T₁ T₂ T₃)).outputs.getIO ident).snd init_s ((cast' ident).mp v) s' := by
+        have: at_least_single_internal init_s := by
+          apply f₆ <;> assumption
+        dsimp [flushed] at *
+        apply f₅ <;> assumption
+      obtain ⟨s', _⟩ := this
+      use s'
+      apply And.intro
+      . assumption
+      . dsimp [flushed] at *
+        unfold φ₄; apply And.intro
+        . apply outputs_preserves_ψ <;> assumption
+        . apply b₂ <;> assumption
+  . --internal rules
+    intro rule mid_i h₁ h₂
+    use init_s
+    apply And.intro
+    . apply existSR_reflexive
+    . dsimp [flushed] at h₁
+      cases h₁
 
 end DataflowRewriter.JoinRewrite
